LambdaLab/Language1/Basic.lean
@@ -1,0 +1,14 @@
+import LambdaLab.Parser.Basic
+
+namespace LambdaLab.Language1
+
+open LambdaLab.Parser
+
+structure Language where
+  Tm : Type
+  Ty : Type
+
+  pTm : LambdaLab.Parser.TruncatingParser Token Tm
+  pTy : LambdaLab.Parser.TruncatingParser Token Ty
+
+end LambdaLab.Language1
