LambdaLab/Parser/Token.lean
@@ -1,0 +1,6 @@
+
+namespace LambdaLab.Parser
+
+abbrev Restricted (P : String → Prop) : Type := { s : String // P s }
+
+end LambdaLab.Parser
