LambdaLab/Parser/Tokenizer1/Basic.lean
@@ -1,0 +1,10 @@
+import LambdaLab.Parser.Basic
+import LambdaLab.Parser.Token
+
+namespace LambdaLab.Parser
+
+--abbrev Token (sep : Char → Bool) := (Restricted (λ s => ∀ c, sep c → c ∉ s))
+
+--def tokenize (sep : Char → Bool) : TruncatingParser Char (List (Token sep)) := sorry
+
+end LambdaLab.Parser
